implementations/ne_list.v
@@ -1,0 +1,46 @@
+Set Implicit Arguments.
+
+Require Import
+  Unicode.Utf8 canonical_names Setoid.
+
+Section contents.
+
+  Variable T: Type.
+
+  Inductive L: Type := one: T → L | cons: T → L → L.
+
+  Fixpoint app (a b: L) {struct a}: L :=
+    match a with
+    | one x => cons x b
+    | cons x y => cons x (app y b)
+    end.
+
+  Fixpoint foldr {R} (o: T → R) (f: T → R → R) (a: L): R :=
+    match a with
+    | one x => o x
+    | cons x y => f x (foldr o f y)
+    end.
+
+  Fixpoint foldr1 (f: T → T → T) (a: L): T :=
+    match a with
+    | one x => x
+    | cons x y => f x (foldr1 f y)
+    end.
+
+  Definition head (l: L): T := match l with one x => x | cons x _ => x end.
+
+  Definition last: L → T := foldr1 (λ x y => y).
+
+  Fixpoint replicate_Sn (x: T) (n: nat): L :=
+    match n with
+    | 0 => one x
+    | S n' => cons x (replicate_Sn x n')
+    end.
+
+End contents.
+
+Fixpoint map `(f: A → B) (l: L A): L B :=
+  match l with
+  | one x => one (f x)
+  | cons h t => cons (f h) (map f t)
+  end.
