theory/monoid_normalization.v
@@ -1,0 +1,127 @@
+Require Import Setoid Morphisms Program Omega Unicode.Utf8.
+Require Import abstract_algebra ua_packed.
+Require universal_algebra varieties.monoid.
+
+Notation msig := varieties.monoid.sig.
+Notation Op := (universal_algebra.Op msig False).
+Notation App := (universal_algebra.App msig False _ _).
+
+Import universal_algebra.
+
+Section contents.
+
+  (* Ideally, we would like to operate exclusively on the universal term representation(s).
+   If Coq had decent support for dependent pattern matching, this would be no problem.
+   Unfortunately, Coq does not, and so we resort to defining an ad-hoc data type for
+   monoidal expressions, with nasty conversions to and from the universal term
+   representation(s): *)
+
+  Context (V: Type).
+
+  Notation uaTerm := (universal_algebra.Term0 msig V tt).
+  Notation Applied := (@ua_packed.Applied msig V tt).
+
+  Inductive Term := Var (v: V) | Unit | Comp (x y: Term).
+
+  Fixpoint to_ua (e: Term): Applied :=
+    match e with
+    | Var v => ua_packed.AppliedVar msig v tt
+    | Unit => ua_packed.AppliedOp msig monoid.one (ua_packed.NoMoreArguments msig tt)
+    | Comp x y => ua_packed.AppliedOp msig monoid.mult
+       (MoreArguments msig tt _ (to_ua x) (MoreArguments msig tt _ (to_ua y) (NoMoreArguments msig tt)))
+    end.
+
+  Definition from_ua (t: Applied): { r: Term | to_ua r ≡ t }.
+  Proof with reflexivity.
+   change ((fun s => match s return ua_packed.Applied msig s → Type with
+     tt => fun t => { r | to_ua r ≡ t } end) tt t).
+   apply better_Applied_rect.
+    simpl.
+    intros []; simpl.
+     intros.
+     exists (Comp (` (fst (forallSplit msig _ _ X)))
+       (` ((fst (forallSplit msig _ _ (snd (forallSplit msig _ _ X))))))).
+     do 3 dependent destruction x.
+     simpl in *.
+     destruct X. destruct p, s. destruct s0.
+     simpl. subst...
+    exists Unit.
+    dependent destruction x...
+   intros v [].
+   exists (Var v)...
+  Defined.
+
+  Fixpoint measure (e: Term): nat :=
+    match e with
+    | Var v => 0%nat
+    | Unit => 1%nat
+    | Comp x y => S (2 * measure x + measure y)
+    end.
+
+  Context `{Monoid M}.
+
+  Notation eval vs := (universal_algebra.eval msig (λ _ => (vs: V → M))).
+
+  Program Fixpoint internal_simplify (t: Term) {measure (measure t)}:
+      { r: Term | Π v, eval v (curry (to_ua r)) = eval v (curry (to_ua t)) } :=
+    match t with
+    | Var _ => t
+    | Unit => t
+    | Comp Unit y => internal_simplify y
+    | Comp x Unit => internal_simplify x
+    | Comp ((Var _) as x) y => Comp x (internal_simplify y)
+    | Comp (Comp x y) z => internal_simplify (Comp x (Comp y z))
+    end.
+
+  Solve Obligations using (program_simpl; simpl; try reflexivity; omega).
+
+  Next Obligation. simpl. apply reflexivity. Qed.
+
+  Next Obligation.
+   destruct internal_simplify.
+   simpl.
+   rewrite e0.
+   transitivity (mon_unit & universal_algebra.eval msig (λ _ => v) (curry (to_ua y))).
+    symmetry.
+    apply left_identity.
+   reflexivity.
+  Qed.
+
+  Next Obligation.
+   destruct internal_simplify.
+   simpl.
+   rewrite e0.
+   transitivity (universal_algebra.eval msig (λ _ => v) (curry (to_ua x)) & mon_unit).
+    symmetry.
+    apply right_identity.
+   reflexivity.
+  Qed.
+
+  Next Obligation. destruct internal_simplify. simpl. rewrite e0. reflexivity. Qed.
+  Next Obligation. destruct internal_simplify. simpl. rewrite e0. simpl. apply associativity. Qed.
+
+  Program Definition simplify (t: uaTerm): { r: uaTerm | Π v, eval v r = eval v t } :=
+    curry (to_ua (internal_simplify (from_ua (decode0 t)))).
+
+  Next Obligation.
+   destruct @internal_simplify. simpl.
+   destruct @from_ua in e0. simpl in *.
+   rewrite e0.
+   rewrite e1.
+   rewrite @curry_decode0.
+   reflexivity.
+  Qed.
+
+  (* This would be a nice theorem to prove:
+
+  Require varieties.open_terms.
+
+  Instance: Equiv V := eq.
+
+  Goal Π (x y: uaTerm), open_terms.ee msig msig monoid.Laws (ne_list.one tt) x y →
+   ` (simplify x) ≡ ` (simplify y).
+  Proof.
+
+  *)
+
+End contents.
