theory/ua_homomorphisms.v
@@ -1,0 +1,188 @@
+Set Automatic Introduction.
+
+Require
+  Unicode.Utf8.
+Require Import
+  Morphisms Setoid Program
+  canonical_names abstract_algebra
+  universal_algebra.
+
+Section contents. Variable σ: Signature.
+
+  Notation OpType := (OpType (sorts σ)).
+
+  Section homo.
+
+  Context
+    (A B: sorts σ → Type)
+    `{ea: Π a, Equiv (A a)} `{eb: Π a, Equiv (B a)}
+    `{ai: AlgebraOps σ A} `{bi: AlgebraOps σ B}.
+
+  Section with_f. Context (f: Π a, A a → B a).
+
+    Implicit Arguments f [[a]].
+
+    Fixpoint Preservation {n: OpType}: op_type A n → op_type B n → Prop :=
+      match n with
+      | ne_list.one d => λ o o' => f o = o'
+      | ne_list.cons x y => λ o o' => Π x, Preservation (o x) (o' (f x))
+      end.
+
+    Class HomoMorphism: Prop :=
+      { homo_proper:> Π a, Setoid_Morphism (@f a)
+      ; preserves: Π (o: σ), Preservation (ai o) (bi o)
+      ; homo_source_algebra: Algebra σ A
+      ; homo_target_algebra: Algebra σ B }.
+
+    Context `{Π i, Equivalence (ea i)} `{Π i, Equivalence (eb i)} `{Π a, Setoid_Morphism (@f a)}.
+
+    Global Instance Preservation_proper n:
+      Proper (op_type_equiv _ _ _ ==> op_type_equiv _ B n ==> iff) (@Preservation n).
+        (* todo: use equiv in the signature and see why things break *)
+    Proof with auto.
+     induction n; simpl; intros x y E x' y' E'.
+      split; intro F. rewrite <- E, <- E'... rewrite E, E'...
+     split; simpl; intros; apply (IHn _ _ (E _ _ (reflexivity _)) _ _ (E' _ _ (reflexivity _)))...
+    Qed.
+
+    Global Instance Preservation_proper'' n:
+      Proper (eq ==> equiv ==> iff) (@Preservation n).
+    Proof with auto.
+     induction n; simpl; intros x y E x' y' E'.
+      split; intro F. rewrite <- E, <- E'... rewrite E, E'...
+     split; simpl; intros.
+      subst.
+      apply (IHn (y x0) (y x0) eq_refl (y' (f x0)) (x' (f x0)) ).
+       symmetry.
+       apply E'.
+       reflexivity.
+      apply H2.
+     subst.
+     apply (IHn (y x0) (y x0) eq_refl (y' (f x0)) (x' (f x0)) ).
+      symmetry.
+      apply E'.
+      reflexivity.
+     apply H2.
+    Qed. (* todo: evil, get rid of *)
+
+  End with_f.
+
+  Lemma Preservation_proper' (f g: Π a, A a → B a)
+   `{Π i, Equivalence (ea i)} `{Π i, Equivalence (eb i)} `{Π a, Setoid_Morphism (@f a)}:
+    (Π a (x: A a), f a x = g a x) → (Π (n: OpType) x y, Proper equiv x → Proper equiv y →
+      @Preservation f n x y →
+      @Preservation g n x y).
+  Proof.
+     induction n.
+      simpl.
+      intros.
+      rewrite <- H5.
+      symmetry.
+      intuition.
+     simpl.
+     intros.
+     apply IHn.
+       apply H3. reflexivity.
+      apply H4. reflexivity.
+     assert (y (g _ x0) = y (f _ x0)).
+      apply H4.
+      symmetry.
+      apply H2.
+     apply (Preservation_proper'' f n (x x0) (x x0) eq_refl _ _ H6).
+     apply H5.
+    Qed.
+
+    Lemma HomoMorphism_Proper: Proper ((λ f g => Π a x, f a x = g a x) ==> iff) HomoMorphism.
+      (* todo: use pointwise_thingy *)
+    Proof with try apply _; intuition.
+     constructor; intros [? ? ? ?]; simpl in *.
+      repeat constructor...
+       repeat intro.
+       do 2 rewrite <- H.
+       rewrite H0...
+      apply (Preservation_proper' x y H (σ o) (ai o) (bi o))...
+     repeat constructor...
+      repeat intro.
+      do 2 rewrite H.
+      rewrite H0...
+     assert (Π (a : sorts σ) (x0 : A a), y a x0 = x a x0). symmetry. apply H.
+     apply (Preservation_proper' y x H0 (σ o) (ai o) (bi o))...
+    Qed.
+
+End homo.
+
+  Global Instance id_homomorphism A
+    `{Π a, Equiv (A a)} {ao: AlgebraOps σ A} `{!Algebra σ A}: HomoMorphism _ _ (λ _ => id).
+  Proof with try apply _; intuition.
+   constructor; intros...
+   generalize (ao o).
+   induction (σ o); simpl...
+   reflexivity.
+  Qed.
+
+  Global Instance compose_homomorphisms A B C f g
+    `{Π a, Equiv (A a)} `{Π a, Equiv (B a)} `{Π a, Equiv (C a)}
+    {ao: AlgebraOps σ A} {bo: AlgebraOps σ B} {co: AlgebraOps σ C}
+    {gh: HomoMorphism A B g} {fh: HomoMorphism B C f}: HomoMorphism A C (λ a => f a ∘ g a).
+  Proof with try apply _; auto.
+   pose proof (homo_source_algebra _ _ g).
+   pose proof (homo_target_algebra _ _ g).
+   pose proof (homo_target_algebra _ _ f).
+   constructor; intros...
+   generalize (ao o) (bo o) (co o) (preserves _ _ g o) (preserves _ _ f o).
+   induction (σ o); simpl; intros; unfold compose.
+    rewrite H5...
+   apply (IHo0 _ (o2 (g _ x)))...
+  Qed.
+
+Implicit Arguments inverse [[A] [B] [Inverse]].
+
+  Lemma invert_homomorphism A B f
+    `{Π a, Equiv (A a)} `{Π a, Equiv (B a)}
+    {ao: AlgebraOps σ A} {bo: AlgebraOps σ B}
+    {fh: HomoMorphism A B f}
+    `{inv: Π a, Inverse (f a)}:
+    (Π a, Bijective (f a)) →
+    HomoMorphism A B f → HomoMorphism B A inv.
+  Proof with try assumption; try apply _.
+   intros.
+   destruct H2.
+   constructor...
+    intro. fold (inverse (f a)). apply _.
+   intro.
+   generalize (ao o) (bo o) (preserves _ _ f o)
+     (algebra_propers o: Proper equiv (ao o)) (algebra_propers o: Proper equiv (bo o)).
+   induction (σ o); simpl.
+    intros.
+    apply (injective (f t)).
+    pose proof (surjective (f t) o1).
+    transitivity o1...
+    symmetry...
+   intros P Q R S T x.
+   apply IHo0.
+     specialize (R (inv t x)).
+     pose proof (surjective (f t) x) as E.
+     rewrite E in R.
+     assumption.
+    apply S. reflexivity.
+   apply T. reflexivity.
+  Qed.
+
+
+(*
+    Instance eval_morphism `{Algebra σ}  A {V} (v: Vars σ A V):
+      HomoMorphism (Term0 σ V) A (λ _ => eval σ v).
+    Proof.
+     constructor; repeat intro; try apply _.
+     unfold AlgebraOps_instance_0.
+     generalize (algebra_propers o: eval v (Op V o) = H o).
+     generalize (Op V o) (H o).
+     induction (operation_type σ o); simpl; repeat intro.
+      assumption.
+     apply IHo0. simpl.
+     apply H1.
+     destruct H0. reflexivity.
+    Qed.
+*)
+
+End contents.
