theory/ua_mapped_operations.v
@@ -1,0 +1,55 @@
+Require Import
+  Setoid Morphisms
+  Unicode.Utf8
+  canonical_names
+  universal_algebra.
+
+Section contents.
+
+  Variable Sorts: Set.
+
+  Section map_op.
+
+    (* Given maps between two realizations of the sorts, there are maps between the corresponding op_types*)
+
+    Context {A B: Sorts → Type}
+      `{Π a, Equiv (A a)} `{Π a, Equiv (B a)}
+      (ab: Π a, A a → B a)
+      (ba: Π a, B a → A a)
+      `{Π a, Proper (equiv ==> equiv) (ab a)}
+      `{Π a, Proper (equiv ==> equiv) (ba a)}.
+
+    Fixpoint map_op {o: OpType Sorts}: op_type A o → op_type B o :=
+      match o return op_type A o → op_type B o with
+      | ne_list.one u => ab u
+      | ne_list.cons _ _ => λ x y => map_op (x (ba _ y))
+      end.
+
+    Global Instance map_op_proper o: Proper ((=) ==> (=)) (@map_op o).
+    Proof. unfold equiv. induction o; simpl; firstorder. Qed.
+      (* todo: can't we make this nameless? *)
+
+  End map_op.
+
+  (* If the maps between the sorts are eachother's inverse, then so are the two generated op_type maps: *)
+
+  Context {A B: Sorts → Type} {e: Π a, Equiv (B a)} `{Π b, Equivalence (e b)} 
+   (ab: Π a, A a → B a) (ba: Π a, B a → A a).
+
+  Implicit Arguments ab [a].
+  Implicit Arguments ba [a].
+
+   Context `(iso: Π a (x: B a), ab (ba x) = x).
+
+  Lemma map_iso o (x: op_type B o) (xproper: Proper (=) x):
+    map_op ab ba (map_op ba ab x) = x.
+  Proof with auto; try reflexivity.
+   induction o; simpl; intros...
+   intros x0 y H0.
+   change (map_op ab ba (map_op ba ab (x (ab (ba x0)))) = x y).
+   transitivity (x (ab (ba x0))).
+    apply IHo, xproper...
+   apply xproper. rewrite iso, H0...
+  Qed.
+
+End contents.
